%%\documentclass[aip,jcp]{revtex4-1}
\documentclass[aip
, pra
, showpacs
, aps
%, twocolumn
, onecolumn
, groupedaddress
, floatfix
%, preprint
]{revtex4}
%]{revtex4-1}
\usepackage{graphicx, amsbsy, bm, dcolumn, amsmath}
\usepackage{currfile}
\usepackage{datetime}

\newcommand{\etal}{{\em et~al.\/}}
\newcommand{\beq}{\begin{equation}}
\newcommand{\eeq}{\end{equation}}
\newcommand{\barr}{\begin{array}}
\newcommand{\earr}{\end{array}}
\newcommand{\JM}{\mbox{\tiny{JM}}}
\newcommand{\Kato}{\mbox{\tiny{Kato}}}
\newcommand{\vare}{\varepsilon}
\newcommand{\phiH}{\phi^{\mbox{\tiny{H}}}}



\newcommand{\isum}%
{\mathop{\hbox{$\displaystyle\sum\kern-13.2pt\int\kern1.5pt$}}}

\begin{document}

\fontsize{12}{15}

\title {Explicitly correlated $J$-matrix method}

\author{Dmitry A. Konovalov}
\affiliation{ARC Centre for Antimatter-Matter Studies}
\affiliation{Discipline of Information Technology, School of Business,
James Cook University, Townsville, Queensland 4811, Australia}

\date{\today, \currenttime}

\begin{abstract}
TODO

\end{abstract}

\pacs{34.80.Dp} %34.80.Dp	Atomic excitation and ionization
\maketitle
The current file is: \currfilename.

\section{INTRODUCTION}

\section{THEORY}
\beq
x \equiv r_< = \min(r_1, r_2), \ \ y \equiv r_> = \max(r_1, r_2),
\eeq
\beq
H = k_1 + k_2 + v_1 + v_2 + v_{12},
\eeq
\beq
k_i = -1/2 d^2/dr^2_i, \ \ v_i = - Z/r_i, \ \ v_{12} = 1/r_>,
\eeq
For symmetric case
\beq
\Phi_{ab}(r_1, r_2) = P_a(x) P_b(y), \ \ \Phi_{ab}(r_1, r_2) = \Phi_{ab}(r_2, r_1),
\eeq
\beq
\Phi_{aa}(r_1, r_2) \equiv P_a(r_1) P_a(r_2),
\eeq
For anti-symmetric case, $a \neq b$,
\beq
??? \ \  \Phi_{ab}(r_1, r_2) = P_a(r_<) P_b(r_>) - P_b(r_<) P_a(r_>),
\eeq
Normalization
\beq \barr{l}
\int_0^\infty dr_1 \int_0^\infty dr_2 \Phi_{ab}(r_1, r_2) \Phi_{a'b'}(r_1, r_2)
=\int_0^\infty dr_1 \int_0^\infty dr_2 P_a(x) P_b(y) P_{a'}(x)  P_{b'}(y)=\\
= \int_0^\infty dr_1  \int_0^{r_1} dr_2 P_a(r_2) P_b(r_1) P_{a'}(r_2) P_{b'}(r_1)
+\int_0^\infty dr_1  \int_{r_1}^\infty dr_2 P_a(r_1) P_b(r_2) P_{a'}(r_1) P_{b'}(r_2)  =\\
= 2 \int_0^\infty dr_1  P_b(r_1) P_{b'}(r_1) \int_0^{r_1} dr_2 P_a(r_2) P_{a'}(r_2)
\earr \eeq
\beq
\int_0^\infty dr_1  \int_{r_1}^\infty dr_2 f(r_1, r_2) \equiv \int_0^\infty dr_2  \int_0^{r_2} dr_1 f(r_1, r_2)
= \int_0^\infty dr_1  \int_0^{r_1} dr_2 f(r_1 \rightleftharpoons r_2)
\eeq
\beq \barr{l}
\int_0^\infty dr_1  \int_{r_1}^\infty dr_2 P_a(r_1) P_b(r_2) P_{a'}(r_1) P_{b'}(r_2)
\equiv \int_0^\infty dr_2  \int_0^{r_2} dr_1 [...] =\\
= [r_1 \rightleftharpoons r_2]
=\int_0^\infty dr_1  \int_0^{r_1} dr_2 P_a(r_2) P_b(r_1) P_{a'}(r_2) P_{b'}(r_1)
\earr \eeq

\subsection{Kinetic energy}
\beq
\partial x / \partial r_1 = \theta(r_2 - r_1), \ \
\partial x / \partial r_2 = \theta(r_1 - r_2),
\eeq
\beq
\partial y / \partial r_1 = \theta(r_1 - r_2), \ \
\partial y / \partial r_2 = \theta(r_2 - r_1),
\eeq
\beq
d \theta(z) / d z = \delta(z), \ \ \delta(\alpha z) = \delta(z)/ |\alpha|
\eeq
\beq
\theta(r_2-r_1) + \theta(r_1-r_2)\equiv 1,
 \ \ \ \theta(r_2-r_1) \theta(r_1-r_2)\equiv 0
\eeq
\beq
\theta(r_2-r_1)= 1 -\theta(r_1-r_2), \ \
\frac{\partial}{\partial r_1} \theta(r_2-r_1) = -\frac{\partial}{\partial r_1} \theta(r_1-r_2) ,
\eeq
\beq \barr{l}
\frac{\partial^2}{\partial r_1^2} P_a(x) P_b(y)
=\frac{\partial}{\partial r_1} [ \frac{\partial P_a(x)}{\partial r_1} P_b(y)
+ P_a(x) \frac{\partial P_b(y)}{\partial r_1} ] =\\
=\frac{\partial}{\partial r_1} [ \theta(r_2-r_1) P'_a(x) P_b(y)
 + \theta(r_1-r_2) P_a(x) P'_b(y)]=\\
=\theta(r_2-r_1) P''_a(x) P_b(y) + \theta(r_1-r_2) P_a(x) P''_b(y)
+\delta(r_1-r_2) [P_a(r) P'_b(r) - P'_a(r) P_b(r)]
\earr \eeq

\beq \barr{l}
\frac{\partial^2}{\partial r_2^2} P_a(x) P_b(y)
=\frac{\partial}{\partial r_1} [ \frac{\partial P_a(x)}{\partial r_1} P_b(y)
+ P_a(x) \frac{\partial P_b(y)}{\partial r_1} ] =\\
=\theta(r_1-r_2) P''_a(x) P_b(y) + \theta(r_2-r_1) P_a(x) P''_b(y)
+\delta(r_1-r_2) [P_a(r) P'_b(r) - P'_a(r) P_b(r)]
\earr \eeq

\beq
[\frac{\partial^2}{\partial r_1^2} + \frac{\partial^2}{\partial r_2^2}] P_a(x) P_b(y)
= P''_a(x) P_b(y) + P_a(x) P''_b(y)
+ 2 \delta(r_1-r_2) [P_a(r) P'_b(r) - P'_a(r) P_b(r)]
\eeq
For $x=\ln(y)$, $y=c+r$, $dx/dr=1/y$
\beq
d/dr P(r) = d/dr [\sqrt{y} F(x)] = \frac{1}{2} y^{-1/2} F(x) + y^{1/2} \frac{dx}{dr} F'(x) =
y^{-1/2} [\frac{1}{2} F(x) + F'(x)]
\eeq
\beq
[P_a(r) P'_b(r) - P'_a(r) P_b(r)] = [F_a(x) F'_b(x) - F'_a(x) F_b(x)]
\eeq


\beq \barr{l}
\int_0^\infty dr_1 \int_0^\infty dr_2 \Phi_{ab}(r_1, r_2) [\frac{\partial^2}{\partial r_1^2} \Phi_{a'b'}(r_1, r_2)]
=\\
= \int_0^\infty dr_1  \int_0^{r_1} dr_2 P_a(r_2) P_b(r_1) [\frac{\partial^2}{\partial r_1^2} P_{a'}(r_2) P_{b'}(r_1)] +\\
\ \ \ +\int_0^\infty dr_1  \int_{r_1}^\infty dr_2 P_a(r_1) P_b(r_2) [\frac{\partial^2}{\partial r_1^2} P_{a'}(r_1) P_{b'}(r_2)]=\\
= \int_0^\infty dr_1  \int_0^{r_1} dr_2 P_a(r_2) P_b(r_1)
[\frac{\partial^2}{\partial r_1^2} + \frac{\partial^2}{\partial r_2^2} ]
P_{a'}(r_2) P_{b'}(r_1)
\earr \eeq
the second term was converted via
\beq \barr{l}
\int_0^\infty dr_1  \int_{r_1}^\infty dr_2 P_a(r_1) P_b(r_2) [\frac{\partial^2}{\partial r_1^2} P_{a'}(r_1) P_{b'}(r_2)]
= \int_0^\infty dr_2  \int_0^{r_1} dr_1 [...] =\\
= [r_1 \rightleftharpoons r_2]
=\int_0^\infty dr_1  \int_0^{r_1} dr_2 P_a(r_2) P_b(r_1) [\frac{\partial^2}{\partial r_2^2} P_{a'}(r_2) P_{b'}(r_1)]
\earr \eeq

\beq \barr{l}
\int_0^\infty dr_1 \int_0^\infty dr_2 \Phi_{ab}(r_1, r_2)
[\frac{1}{2}\frac{\partial^2}{\partial r_1^2} + \frac{1}{2} \frac{\partial^2}{\partial r_2^2}]\Phi_{a'b'}(r_1, r_2)
=\\
=\int_0^\infty dr_1  \int_0^{r_1} dr_2 P_a(r_2) P_b(r_1)
[\frac{\partial^2}{\partial r_1^2} + \frac{\partial^2}{\partial r_2^2} ]
P_{a'}(r_2) P_{b'}(r_1)=\\
=\int_0^\infty dr_1  P_b(r_1) P_{b'}(r_1) \int_0^{r_1} dr_2 P_a(r_2) P''_{a'}(r_2)
+\int_0^\infty dr_1  P_b(r_1) P''_{b'}(r_1) \int_0^{r_1} dr_2 P_a(r_2) P_{a'}(r_2)
\earr \eeq

\subsection{Potential Energy}
Potential energy for $v_{12}=1/y$
\beq \barr{l}
\int_0^\infty dr_1 \int_0^\infty dr_2 \Phi_{ab}(r_1, r_2) \frac{1}{y} \Phi_{a'b'}(r_1, r_2)
= 2 \int_0^\infty dr_1  P_b(r_1) P_{b'}(r_1) \frac{1}{r_1} \int_0^{r_1} dr_2 P_a(r_2) P_{a'}(r_2)
\earr \eeq
Potential energy for $v_{1}$
\beq \barr{l}
\int_0^\infty dr_1 \int_0^\infty dr_2 \Phi_{ab}(r_1, r_2) \frac{1}{r_1} \Phi_{a'b'}(r_1, r_2)
=\int_0^\infty dr_1 \int_0^\infty dr_2 P_a(x) P_b(y) \frac{1}{r_1} P_{a'}(x) P_{b'}(y)=\\
= \int_0^\infty dr_1  \int_0^{r_1} dr_2 P_a(r_2) P_b(r_1) \frac{1}{r_1} P_{a'}(r_2) P_{b'}(r_1)
+\int_0^\infty dr_1  \int_{r_1}^\infty dr_2 P_a(r_1) P_b(r_2) \frac{1}{r_1} P_{a'}(r_1) P_{b'}(r_2)  =\\
= \int_0^\infty dr_1  P_b(r_1) \frac{1}{r_1} P_{b'}(r_1) \int_0^{r_1} dr_2 P_a(r_2) P_{a'}(r_2)
+ \int_0^\infty dr_1  P_b(r_1) P_{b'}(r_1) \int_0^{r_1} dr_2 P_a(r_2) \frac{1}{r_2} P_{a'}(r_2)
\earr \eeq


\section{RESULTS}
TODO
\section{CONCLUSIONS}
TODO


\begin{acknowledgments}
\end{acknowledgments}



\bibliographystyle{apsrev}
\bibliography{..//bibtex//qm_references}
%\bibliography{qm_references}
\end{document}
